WIP: sc steps

src/mapping/PStoRMW.v
@@ -61,24 +61,52 @@ Module PStoRMW.
         (PROMISES3: eu3.(RMWExecUnit.local).(Local.promises) = bot)
   .
 
+  Variant sim_thread_sl (tid: Ident.t) (n: Time.t) (after_sc: bool)
+    (gl_ps: PSGlobal.t) (mem_arm: Memory.t):
+    forall (sl_ps: {lang: language & Language.state lang} * PSLocal.t)
+           (sl_arm: RMWState.t (A:=View.t (A:=unit)) * Local.t (A:=unit)), Prop :=
+    | sim_thread_sl_intro
+        st_ps lc_ps st_arm lc_arm
+        (SIM_THREAD: sim_thread_exec tid n after_sc
+                       (PSThread.mk _ st_ps lc_ps gl_ps) (RMWExecUnit.mk st_arm lc_arm mem_arm)):
+      sim_thread_sl tid n after_sc gl_ps mem_arm
+        (existT _ lang_ps st_ps, lc_ps) (st_arm, lc_arm)
+  .
+
+  Variant sim (n: Time.t) (after_sc: bool) (c: PSConfiguration.t) (m: RMWMachine.t): Prop :=
+    | sim_intro
+        m1
+        (PROMISE_STEPS: rtc (RMWMachine.step RMWExecUnit.promise_step) m m1)
+        (SIM_THREADS:
+          forall tid,
+            opt_rel
+              (sim_thread_sl tid n after_sc c.(PSConfiguration.global) m.(RMWMachine.mem))
+              (IdentMap.find tid c.(PSConfiguration.threads))
+              (IdMap.find tid m.(RMWMachine.tpool)))
+        (SIM_SC: forall loc,
+            PSTime.le (c.(PSConfiguration.global).(PSGlobal.sc) loc) (ntt n))
+  .
+
+
   Lemma sim_thread_exec_sc
         tid n th1_ps eu
-        (SIM: sim_thread_exec tid n false th1_ps eu)
+        (SIM1: sim_thread_exec tid n false th1_ps eu)
         (SC1: forall loc, PSTime.le (th1_ps.(PSThread.global).(PSGlobal.sc) loc) (ntt n))
         (LC_WF1_PS: PSLocal.wf (PSThread.local th1_ps) (PSThread.global th1_ps))
         (GL_WF1_PS: PSGlobal.wf (PSThread.global th1_ps))
         (WF_ARM: RMWLocal.wf tid (RMWExecUnit.local eu) (RMWExecUnit.mem eu)):
     exists th2_ps,
       (<<STEPS_PS: rtc (@PSThread.tau_step _) th1_ps th2_ps>>) /\
-      ((<<SIM_AFTER: sim_thread_exec tid n true th2_ps eu>>) \/
+      ((<<SIM2: sim_thread_exec tid n true th2_ps eu>>) /\
+       (<<SC2: forall loc, PSTime.le (th2_ps.(PSThread.global).(PSGlobal.sc) loc) (ntt n)>>) \/
        exists e_ps th3_ps,
          (<<STEP_PS: PSThread.step e_ps th2_ps th3_ps>>) /\
          (<<FAILURE: ThreadEvent.get_machine_event e_ps = MachineEvent.failure>>)).
   Proof.
-    inv SIM.
+    inv SIM1.
     exploit (dmbsy_le_cases (A:=unit)); try exact STEPS3. i. des.
     { exploit (dmbsy_le_cases (A:=unit)); try exact STEPS2. i. des.
-      { esplits; try refl. left. econs; eauto. }
+      { esplits; try refl. left. split; ss. econs; eauto. }
       exploit rtc_n1; try exact STEPS_DMBSY1.
       { eapply RMWExecUnit.dmbsy_dmbsy_exact. eauto. }
       intro STEPS_EXACT.
@@ -92,7 +120,8 @@ Module PStoRMW.
         ii. rewrite PROMISES3, Promises.lookup_bot in *. ss.
       }
       i. des; [|esplits; eauto].
-      esplits; eauto. left. econs.
+      esplits; eauto. left. split; ss.
+      econs.
       - etrans; [exact STEPS1|].
         eapply rtc_mon; try eapply RMWExecUnit.pf_state_step_state_step.
         eapply rtc_mon; try eapply RMWExecUnit.dmbsy_exact_state_step.
@@ -122,7 +151,8 @@ Module PStoRMW.
         ii. rewrite PROMISES3, Promises.lookup_bot in *. ss.
       }
       i. des; [|esplits; eauto].
-      esplits; eauto. left. econs.
+      esplits; eauto. left. split; ss.
+      econs.
       - etrans; [exact STEPS1|].
         eapply rtc_mon; try eapply RMWExecUnit.pf_state_step_state_step.
         eapply rtc_mon; try eapply RMWExecUnit.dmbsy_exact_state_step.
@@ -138,29 +168,43 @@ Module PStoRMW.
     }
   Qed.
 
-  Variant sim_thread_sl (tid: Ident.t) (n: Time.t) (after_sc: bool)
-    (gl_ps: PSGlobal.t) (mem_arm: Memory.t):
-    forall (sl_ps: {lang: language & Language.state lang} * PSLocal.t)
-           (sl_arm: RMWState.t (A:=View.t (A:=unit)) * Local.t (A:=unit)), Prop :=
-    | sim_thread_sl_intro
-        st_ps lc_ps st_arm lc_arm
-        (SIM_THREAD: sim_thread_exec tid n after_sc
-                       (PSThread.mk _ st_ps lc_ps gl_ps) (RMWExecUnit.mk st_arm lc_arm mem_arm)):
-      sim_thread_sl tid n after_sc gl_ps mem_arm
-        (existT _ lang_ps st_ps, lc_ps) (st_arm, lc_arm)
-  .
-
-  Variant sim (n: Time.t) (c: PSConfiguration.t) (m: RMWMachine.t): Prop :=
-    | sim_intro
-        m1
-        (PROMISE_STEPS: rtc (RMWMachine.step RMWExecUnit.promise_step) m m1)
-        (SIM_THREADS:
-          forall tid,
-            opt_rel
-              (sim_thread_sl tid n true c.(PSConfiguration.global) m.(RMWMachine.mem))
-              (IdentMap.find tid c.(PSConfiguration.threads))
-              (IdMap.find tid m.(RMWMachine.tpool)))
-        (SIM_SC: forall loc,
-            PSTime.le (c.(PSConfiguration.global).(PSGlobal.sc) loc) (ntt n))
-  .
+  Lemma sim_sc
+        n c1 m
+        (SIM1: sim n false c1 m)
+        (WF1_PS: PSConfiguration.wf c1)
+        (WF_ARM: RMWMachine.rmw_wf m):
+    exists c2,
+      (<<STEPS_PS: rtc PSConfiguration.tau_step c1 c2>>) /\
+      ((<<SIM2: sim n true c2 m>>) \/
+       exists tid c3,
+         (<<STEP: PSConfiguration.step MachineEvent.failure tid c2 c3>>)).
+  Proof.
+    inv SIM1.
+    assert (exists tids,
+               (<<IN: forall tid (IN: List.In tid tids),
+                   opt_rel
+                     (sim_thread_sl tid n false c1.(PSConfiguration.global) m.(RMWMachine.mem))
+                     (IdentMap.find tid c1.(PSConfiguration.threads))
+                     (IdMap.find tid m.(RMWMachine.tpool))>>) /\
+               (<<OUT: forall tid (OUT: ~ List.In tid tids),
+                   opt_rel
+                     (sim_thread_sl tid n true c1.(PSConfiguration.global) m.(RMWMachine.mem))
+                     (IdentMap.find tid c1.(PSConfiguration.threads))
+                     (IdMap.find tid m.(RMWMachine.tpool))>>)).
+    { admit.
+    }
+    des. clear SIM_THREADS.
+    revert c1 WF1_PS SIM_SC IN OUT.
+    induction tids; i.
+    { esplits; try refl. left. econs; eauto. }
+    destruct c1 as [ths1 gl1].
+    exploit (IN a); ss; auto. intro SIM_THREAD.
+    destruct (IdentMap.find a ths1) as [[[lang st1] lc1]|] eqn:FIND_PS; cycle 1.
+    { inv SIM_THREAD.
+      eapply IHtids; try exact WF1_PS; eauto. s. i.
+      destruct (Ident.eq_dec tid a).
+      { subst. rewrite FIND_PS, <- H. ss. }
+      eapply (OUT tid). ii. des; eauto.
+    }
+  Admitted.
 End PStoRMW.
